Prove reorder's simulation part 1: load

src/lib/Basic.v
@@ -5,6 +5,8 @@ Require Import FMapPositive.
 Require Import FMapFacts.
 Require Import MSetList.
 
+Require Import sflib.
+
 Require Import DataStructure.
 
 Set Implicit Arguments.
@@ -40,6 +42,129 @@ Module IdentMap.
   Include PositiveMap.
   Module Facts := FMapFacts.Facts (PositiveMap).
   Module Properties := FMapFacts.Properties (PositiveMap).
+
+  Inductive lift_rel2 A B (rel:forall (a:A) (b:B), Prop): forall (a:option A) (b:option B), Prop :=
+  | lift_rel2_None:
+      lift_rel2 rel None None
+  | lift_rel2_Some
+      a b (REL: rel a b):
+      lift_rel2 rel (Some a) (Some b)
+  .
+
+  Definition rel2
+             A B (rel: forall (a:A) (b:B), Prop)
+             (ma:t A) (mb:t B): Prop :=
+    forall i, lift_rel2 rel (find i ma) (find i mb).
+
+  Lemma rel2_elim
+        A B C
+        (ab: forall (a:A) (b:B), Prop)
+        (bc: forall (b:B) (c:C), Prop)
+        (ma:t A) (mb:t B) (mc:t C)
+        (AB: rel2 ab ma mb)
+        (BC: rel2 bc mb mc):
+    rel2 (fun a c => exists b, ab a b /\ bc b c) ma mc.
+  Proof.
+    intro. specialize (AB i). specialize (BC i).
+    inv AB; inv BC; try congruence; constructor.
+    rewrite <- H2 in H. inv H.
+    eexists. split; eauto.
+  Qed.
+
+  Lemma rel2_converse
+        A B
+        (ab: forall (a:A) (b:B), Prop)
+        (ma:t A) (mb:t B)
+        (AB: rel2 ab ma mb):
+    rel2 (fun b a => ab a b) mb ma.
+  Proof.
+    intro i. specialize (AB i).
+    inv AB; constructor; auto.
+  Qed.
+
+  Lemma rel2_leaf
+        A B
+        (ab: forall (a:A) (b:B), Prop)
+        (mb:t B)
+        (AB: rel2 ab (Leaf _) mb):
+    is_empty mb.
+  Proof.
+    revert AB. induction mb; intros; simpl; auto.
+    destruct o.
+    { specialize (AB xH). inv AB. }
+    rewrite IHmb1, IHmb2; auto.
+    - intro i. specialize (AB (xI i)). inv AB.
+      rewrite gempty. constructor.
+    - intro i. specialize (AB (xO i)). inv AB.
+      rewrite gempty. constructor.
+  Qed.
+
+  Lemma rel2_intro
+        A B C
+        (ab: forall (a:A) (b:B), Prop)
+        (bc: forall (b:B) (c:C), Prop)
+        (ma:t A) (mc:t C)
+        (AC: rel2 (fun a c => exists b, ab a b /\ bc b c) ma mc):
+    exists mb,
+      <<AB: rel2 ab ma mb>> /\
+      <<BC: rel2 bc mb mc>>.
+  Proof.
+    revert mc AC.
+    induction ma; destruct mc; intros.
+    - exists (Leaf _). split; intro; rewrite ? gempty; constructor.
+    - exists (Leaf _). split; intro; rewrite ? gempty.
+      1: constructor.
+      apply rel2_leaf in AC. apply PositiveMap.is_empty_2 in AC.
+      rewrite PositiveMap.Empty_alt in AC. rewrite AC.
+      constructor.
+    - exists (Leaf _). split; intro; rewrite ? gempty.
+      2: constructor.
+      apply rel2_converse, rel2_leaf in AC. apply PositiveMap.is_empty_2 in AC.
+      rewrite PositiveMap.Empty_alt in AC. rewrite AC.
+      constructor.
+    - exploit IHma1.
+      { intro i. specialize (AC (xO i)).
+        inv AC; rewrite <- H; constructor; auto.
+      }
+      exploit IHma2.
+      { intro i. specialize (AC (xI i)).
+        inv AC; rewrite <- H; constructor; auto.
+      }
+      intros [mb2 MB2] [mb1 MB1]. des.
+      specialize (AC xH). inv AC.
+      + eexists (Node mb1 None mb2).
+        simpl in *. subst.
+        split; intro; destruct i; simpl;
+          try apply AB0; try apply BC0;
+          try apply AB; try apply BC;
+          constructor.
+      + des. eexists (Node mb1 (Some b0) mb2).
+        simpl in *. subst.
+        split; intro; destruct i; simpl;
+          try apply AB0; try apply BC0;
+          try apply AB; try apply BC;
+          constructor; auto.
+  Qed.
+
+  Lemma rel2_implies
+        A B
+        (ab1 ab2: forall (a:A) (b:B), Prop)
+        (IMPLIES: forall a b, ab1 a b -> ab2 a b)
+        (ma:t A) (mb:t B)
+        (AB: rel2 ab1 ma mb):
+    rel2 ab2 ma mb.
+  Proof.
+    intro i. specialize (AB i).
+    inv AB; constructor; auto.
+  Qed.
+
+  Lemma rel2_construct
+        A B (c: A -> B) (ma:t A):
+    rel2 (fun a b => b = c a) ma (map c ma).
+  Proof.
+    intro i. rewrite Facts.map_o.
+    destruct (find i ma); simpl; constructor; auto.
+  Qed.
 
   Definition get_max V (pred: V -> nat) (m:t V): nat :=
     fold
@@ -84,12 +209,3 @@ Notation rtc := (clos_refl_trans _). (* reflexive transitive closure *)
 Notation rc := (clos_refl _). (* reflexive transitive closure *)
 Notation tc := (clos_trans _). (* transitive closure *)
 Hint Immediate rt_step rt_refl t_step.
-
-
-Inductive lift_rel2 A B (rel:forall (a:A) (b:B), Prop): forall (a:option A) (b:option B), Prop :=
-| lift_rel2_None:
-    lift_rel2 rel None None
-| lift_rel2_Some
-    a b (REL: rel a b):
-    lift_rel2 rel (Some a) (Some b)
-.
