src/reorder/Reorder.v
@@ -1,4 +1,6 @@
+Require Import Bool.
 Require Import List.
+Require Import ProofIrrelevance.
 
 Require Import sflib.
 
@@ -14,85 +16,97 @@ Require Import Simulation.
 
 Set Implicit Arguments.
 
-Inductive reorderable: forall (i1 i2:Instr.t), Prop :=
-| reorderable_intro
-    i1 i2
-    (I1NACQ: not (Ordering.weaker Ordering.acquire (Instr.ordering_of i1)))
-    (I2NREL: not (Ordering.weaker Ordering.release (Instr.ordering_of i2)))
-    (LOC: forall loc1 loc2
-            (LOC1: Instr.loc_of i1 = Some loc1)
-            (LOC2: Instr.loc_of i2 = Some loc2),
-        loc1 <> loc2)
-    (REG: RegSet.Empty (RegSet.inter (Instr.regs_of i1) (Instr.regs_of i2))):
-    reorderable i1 i2
-.
+(* TODO: now supporting only the reordering of load and store *)
 
-Inductive reordered_stmt: forall (s1 s2:Stmt.t), Prop :=
-| reordered_instr i:
-    reordered_stmt
+Definition reorderable_message (msg1 msg2:Message.t): bool :=
+  match msg1, msg2 with
+  | Message.rw (RWEvent.read l1 c1 o1) t1,
+    Message.rw (RWEvent.write l2 c2 o2) t2 =>
+    (negb (Loc.eqb l1 l2)) &&
+    (negb (Ordering.ord Ordering.acquire o1)) &&
+    (negb (Ordering.ord Ordering.release o2))
+  | _, _ =>
+    false
+  end.
+
+Definition reorderable_instr (i1 i2:Instr.t): bool :=
+  match i1, i2 with
+  | Instr.load r1 l1 o1,
+    Instr.store l2 v2 o2 =>
+    (negb (Loc.eqb l1 l2)) &&
+    (RegSet.is_empty (RegSet.inter (Instr.regs_of i1) (Instr.regs_of i2))) &&
+    (negb (Ordering.ord Ordering.acquire o1)) &&
+    (negb (Ordering.ord Ordering.release o2))
+  | _, _ =>
+    false
+  end.
+
+Inductive trans_stmt: forall (s1 s2:Stmt.t), Prop :=
+| trans_stmt_instr i:
+    trans_stmt
       (Stmt.instr i)
       (Stmt.instr i)
-| reordered_ite
+| trans_stmt_ite
     cond c11 c12 c21 c22
-    (REORDER1: reordered_stmts c11 c21)
-    (REORDER2: reordered_stmts c12 c22):
-    reordered_stmt
+    (TRANS1: trans_stmts c11 c21)
+    (TRANS2: trans_stmts c12 c22):
+    trans_stmt
       (Stmt.ite cond c11 c12)
       (Stmt.ite cond c21 c22)
-| reordered_dowhile
+| trans_stmt_dowhile
     cond c1 c2
-    (REORDER2: reordered_stmts c1 c2):
-    reordered_stmt
+    (TRANS2: trans_stmts c1 c2):
+    trans_stmt
       (Stmt.dowhile c1 cond)
       (Stmt.dowhile c2 cond)
 
-with reordered_stmts: forall (s1 s2:list Stmt.t), Prop :=
-| reordered_nil:
-    reordered_stmts nil nil
-| reordered_cons
+with trans_stmts: forall (s1 s2:list Stmt.t), Prop :=
+| trans_stmts_nil:
+    trans_stmts nil nil
+| trans_stmts_cons
     s11 s12 s21 s22
-    (REORDER1: reordered_stmt s11 s21)
-    (REORDER2: reordered_stmts s12 s22):
-    reordered_stmts (s11::s12) (s21::s22)
-| reordered_reorder
+    (TRANS1: trans_stmt s11 s21)
+    (TRANS2: trans_stmts s12 s22):
+    trans_stmts (s11::s12) (s21::s22)
+| trans_stmts_reorder
     i1 i2 s1 s2
-    (REORDER1: reorderable i1 i2)
-    (REORDER2: reordered_stmts s1 s2):
-    reordered_stmts
+    (REORDER: reorderable_instr i1 i2)
+    (TRANS: trans_stmts s1 s2):
+    trans_stmts
       ((Stmt.instr i1)::(Stmt.instr i2)::s1)
       ((Stmt.instr i2)::(Stmt.instr i1)::s2)
 .
 
-Scheme reordered_stmt_ind_ := Induction for reordered_stmt Sort Prop
-with reordered_stmts_ind_ := Induction for reordered_stmts Sort Prop.
-Combined Scheme reordered_ind from reordered_stmt_ind_, reordered_stmts_ind_.
+Scheme trans_stmt_ind_ := Induction for trans_stmt Sort Prop
+with trans_stmts_ind_ := Induction for trans_stmts Sort Prop.
+Combined Scheme trans_ind from trans_stmt_ind_, trans_stmts_ind_.
 
-Inductive reordered_prog_thread: forall (text1 text2:Program.thread_t), Prop :=
-| reordered_prog_thread_intro
+Inductive trans_prog_thread: forall (text1 text2:Program.thread_t), Prop :=
+| trans_prog_thread_intro
     s1 s2
-    (REORDERED: reordered_stmts s1 s2):
-    reordered_prog_thread
+    (TRANS: trans_stmts s1 s2):
+    trans_prog_thread
       (Program.thread_mk lang s1)
       (Program.thread_mk lang s2)
 .
 
-Inductive reordered_prog (prog1 prog2:Program.t): Prop :=
-| reordered_prog_intro
-    (REORDERED: forall i, lift_rel2 reordered_prog_thread (IdentMap.find i prog1) (IdentMap.find i prog2))
+Inductive trans_prog (prog1 prog2:Program.t): Prop :=
+| trans_prog_intro
+    (TRANS: IdentMap.rel2 trans_prog_thread prog1 prog2)
 .
 
 Inductive consumed (i2:Instr.t): forall (c1 c2:list Stmt.t), Prop :=
 | consumed_intro
     i1 c1 c2
-    (REORDER1: reorderable i1 i2)
-    (REORDER2: reordered_stmts c1 c2):
+    (REORDER: reorderable_instr i1 i2)
+    (TRANS: trans_stmts c1 c2):
     consumed i2 ((Stmt.instr i1)::(Stmt.instr i2)::c1) ((Stmt.instr i1)::c2)
 .
 
 Inductive sim_thread: forall (e:option ThreadEvent.t) (th1 th2:Thread.t), Prop :=
-| sim_thread_reordered
+| sim_thread_trans
     rs s1 s2
-    (REORDERED: reordered_stmts s1 s2):
+    (TRANS: trans_stmts s1 s2):
     sim_thread
       None
       (Thread.mk lang (State.mk rs s1))
@@ -107,27 +121,44 @@ Inductive sim_thread: forall (e:option ThreadEvent.t) (th1 th2:Thread.t), Prop :
       (Thread.mk lang (State.mk rs2 s2))
 .
 
+Inductive sim_history: forall (b1 b2:list Message.t), Prop :=
+| sim_history_nil:
+    sim_history nil nil
+| sim_history_cons
+    msg b1 b2
+    (HISTORY: sim_history b1 b2):
+    sim_history (b1 ++ [msg]) (b2 ++ [msg])
+| sim_history_reorder
+    msg1 msg2 b1 b2
+    (MSG: reorderable_message msg1 msg2)
+    (HISTORY: sim_history b1 b2):
+    sim_history (b1 ++ [msg1; msg2]) (b2 ++ [msg2; msg1])
+.
+
 Inductive sim_buffer: forall (e:option ThreadEvent.t) (b1 b2:Buffer.t), Prop :=
-| sim_buffer_reordered
-    history inception:
+| sim_buffer_trans
+    history1 history2 inception
+    (HISTORY: sim_history history1 history2):
     sim_buffer
       None
-      (Buffer.mk history inception)
-      (Buffer.mk history inception)
+      (Buffer.mk history1 inception)
+      (Buffer.mk history2 inception)
 | sim_buffer_consumed_observable
-    msg history1 inception2
-    (OBSERVABLE: Message.observable msg = true):
+    msg history1 history2 inception2
+    (HISTORY: sim_history history1 history2)
+    (OBSERVABLE: Message.observable msg):
     sim_buffer
       (Some (Message.get_threadevent msg))
       (Buffer.mk history1 (MessageSet.add msg inception2))
-      (Buffer.mk (history1 ++ [msg]) inception2)
+      (Buffer.mk (history2 ++ [msg]) inception2)
 | sim_buffer_consumed_unobservable
-    msg history1 inception
-    (UNOBSERVABLE: Message.observable msg = false):
+    msg history1 history2 inception
+    (HISTORY: sim_history history1 history2)
+    (UNOBSERVABLE: ~ Message.observable msg):
     sim_buffer
       (Some (Message.get_threadevent msg))
       (Buffer.mk history1 inception)
-      (Buffer.mk (history1 ++ [msg]) inception)
+      (Buffer.mk (history2 ++ [msg]) inception)
 .
 
 Inductive sim_thread_buffer: forall (th1 th2:option Thread.t) (b1 b2:option Buffer.t), Prop :=
@@ -160,31 +191,46 @@ Inductive sim_configuration (c1 c2:Configuration.t): Prop :=
 
 Lemma sim_load_thread
       text_src text_tgt th_tgt
-      (REORDERED: reordered_prog_thread text_src text_tgt)
+      (TRANS: trans_prog_thread text_src text_tgt)
       (TGT: Program.load_thread text_tgt th_tgt):
   exists th_src,
     <<SRC: Program.load_thread text_src th_src>> /\
     <<SIM: sim_thread None th_src th_tgt>>.
 Proof.
-  inv REORDERED; inv TGT.
-  apply ProofIrrelevance.ProofIrrelevanceTheory.EqdepTheory.inj_pair2 in H1. subst.
+  inv TRANS; inv TGT.
+  apply inj_pair2 in H1. subst.
   inv LOAD. exists (Thread.mk lang (State.mk RegFile.init s1)).
   split; repeat constructor; auto.
 Qed.
 
 Lemma sim_load
       prog_src prog_tgt
-      (REORDERED: reordered_prog prog_src prog_tgt):
+      (TRANS: trans_prog prog_src prog_tgt):
   Simulation.LOAD prog_src prog_tgt sim_configuration.
 Proof.
-  inv REORDERED.
-  eexists (Configuration.mk Clocks.init _ Memory.empty []).
-  inv TGT. inv LOAD.
-  split; constructor; simpl; auto.
-  - admit.
-  - admit.
-  - admit.
-Admitted.
+  inv TRANS.
+  repeat intro. inv TGT. inv LOAD.
+  generalize (IdentMap.rel2_elim TRANS0 LOAD0). intro REL2.
+  eapply (IdentMap.rel2_implies
+            (fun text th => exists th', Program.load_thread text th' /\
+                                sim_thread None th' th))
+    in REL2.
+  all: cycle 1.
+  { intros. des. inv H. inv H0. inv LOAD.
+    apply inj_pair2 in H2. subst.
+    repeat econs; eauto.
+  }
+
+  apply IdentMap.rel2_intro in REL2. des.
+  eexists (Configuration.mk Clocks.init mb _ []).
+  repeat econs; simpl; eauto.
+  { apply IdentMap.rel2_construct. }
+  { intro i. rewrite IdentMap.Facts.map_o.
+    specialize (BC i). specialize (MEM i).
+    inv BC; inv MEM; simpl; try constructor; try congruence.
+    repeat econs; eauto.
+  }
+Qed.
 
 Lemma sim_step: Simulation.STEP sim_configuration.
 Proof.
@@ -200,9 +246,9 @@ Admitted.
 
 Definition sim
            prog_src prog_tgt
-           (REORDERED: reordered_prog prog_src prog_tgt) :=
+           (TRANS: trans_prog prog_src prog_tgt) :=
   Simulation.mk
-    (sim_load REORDERED)
+    (sim_load TRANS)
     sim_step
     sim_observable
     sim_terminal.
